verified/psrbits.i.dfy
@@ -112,7 +112,6 @@ lemma lemma_update_psr(oldpsr:word, newmode:word, f:bool, i:bool)
             assert (BitAnd(maskbits, 0x40) != 0) == f by { reveal BitAnd(); }
 
             reveal BitAnd(); reveal_BitOr();
-            reveal WordAligned(); // why?
         }
         f || decode_psr(oldpsr).f;
     }
@@ -141,7 +140,6 @@ lemma lemma_update_psr(oldpsr:word, newmode:word, f:bool, i:bool)
             assert (BitAnd(maskbits, 0x80) != 0) == i by { reveal BitAnd(); }
 
             reveal BitAnd(); reveal_BitOr();
-            reveal WordAligned(); // why?
         }
         i || decode_psr(oldpsr).i;
     }
