verified/sha/sha256.i.dfy
@@ -567,7 +567,8 @@ lemma lemma_SHA256FinalHelper1(
         WordSeqToBytes(ConcatenateSeqs(z.M));
         processed_bytes;
         message + unprocessed_bytes;
-            { lemma_ArrayOffsetConcatenation(unprocessed_bytes, 0, 1, 64); }
+            { lemma_ArrayOffsetConcatenation(unprocessed_bytes, 0, 1, 64);
+              assert unprocessed_bytes[0] == 0x80; }
         message + ([0x80] + unprocessed_bytes[1..64]);
             { lemma_SeqConcatenationIsAssociative(message, [0x80], unprocessed_bytes[1..64]); }
         message + [0x80] + unprocessed_bytes[1..64];
